\documentclass{article}
\usepackage{mathtools}
\usepackage[]{mcode}

\begin{document}
	$
	\begin{pmatrix*}[l]
		D1(1) & D2(1) & 0 & D3(1) & 0 & 0 \\
		D2(1) & D1(2) & D2(2) & 0 & D3(2) & 0 \\
		0 & D2(2) & D1(3) & D2(3) & 0 & D3(3)\\
		D3(1) & 0 & D2(3) & D1(4) & D2(4) & 0 \\
		0 & D3(2) & 0 & D2(4) & D1(5) & D2(5) \\
		0 & 0 & D3(3) & 0 & D2(5) & D1(6)
	\end{pmatrix*}
	$
	
	$
	x_i^{(k+1)} = 
	\frac{1}{D1_i}(b_i-s_i)
	$
	
	$ 
	s_1 = D2_1x^{(k)}_2 + D3_1x_4^{(k)}
	$
	
	$
	s_i =  D2_ix^{(k)}_{i+1} + D2_{i-1}x^{(k)}_{i-1} + D3_ix^{(k)}_{i+3} \text{ } 
	 (i\in\{2,3\})
	$ 
	
	$ 
	s_i = D2_ix^{(k)}_{i+1} + D2_{i-1}x^{(k)}_{i-1} + D3_ix^{(k)}_{i+3} + D3_{i-3}x_{i-3}^{(k)} \text{ } 
		 (4 \leq i \leq n-3)
	$
	
	$ 
	s_i = D2_ix^{(k)}_{i+1} + D2_{i-1}x^{(k)}_{i-1} + D3_{i-3}x^{(k)}_{i-3} \text{ } 
	 (i \in\{n-2,n-1\})
	$
	
	$
	s_n = D2_{n-1}x^{(k)}_{n-1} + D3_{n-3}x^{(k)}_{n-3}
	$
	
	$
	\frac{\parallel x^{(k+1)} - x^{(k)} \parallel _\infty}{\parallel x^{(k+1)} \parallel _\infty} \leq 0.0001
	$	

	$ 
	s_1 = D2_1x^{(k)}_2 + D3_1x_4^{(k)}
	$
	
	$
	s_i =  D2_ix^{(k)}_{i+1} + D2_{i-1}x^{(k+1)}_{i-1} + D3_ix^{(k)}_{i+3} \text{ } 
 (i\in\{2,3\})
	$ 
	
	$ 
	s_i = D2_ix^{(k)}_{i+1} + D2_{i-1}x^{(k+1)}_{i-1} + D3_ix^{(k)}_{i+3} + D3_{i-3}x_{i-3}^{(k+1)} \text{ } 
	 (4 \leq i \leq n-3)
	$
	
	$ 
	s_i = D2_ix^{(k)}_{i+1} + D2_{i-1}x^{(k+1)}_{i-1} + D3_{i-3}x^{(k+1)}_{i-3} \text{ } 
	 (i \in\{n-2,n-1\})
	$
	
	$
	s_n = D2_{n-1}x^{(k+1)}_{n-1} + D3_{n-3}x^{(k+1)}_{n-3}
	$
	
	$
	\ln{\parallel x^{(k)} - x \parallel_\infty} = k\ln{\rho} + \ln{\parallel x^{(0)} - x \parallel_\infty}
	$
\end{document}